Config.v
@@ -1,4 +1,4 @@
-From Coq Require Import String ZArith.
+From Coq Require Import String ZArith CyclicAxioms ZModulo.
 Require FSet Map.
 
 Class VyperConfig := {
@@ -8,6 +8,8 @@ Class VyperConfig := {
   string_map_impl: forall t: Type, Map.class String.string_dec t (string_map t);
   world_state: Type;
   uint256: Type;
+  Z_of_uint256: uint256 -> Z;
+  uint256_of_Z: Z -> uint256;
   storage_lookup: world_state -> string -> option uint256;
 }.
 
@@ -18,6 +20,17 @@ Definition sample_config
       string_map := Map.string_avl_map;
       string_map_impl := Map.string_avl_map_impl;
       world_state := Map.string_avl_map Z;
-      uint256 := Z; (* XXX *)
+      uint256 := Z;
+      Z_of_uint256 := id;
+      uint256_of_Z z := (z mod 2^256)%Z;
       storage_lookup := let _ := Map.string_avl_map_impl in Map.lookup;
    |}.
+
+Definition zero256 {C: VyperConfig} := uint256_of_Z 0%Z.
+Definition one256  {C: VyperConfig} := uint256_of_Z 1%Z.
+
+Definition maybe_uint256_of_Z {C: VyperConfig} (z: Z)
+:= let u := uint256_of_Z z in
+   if (Z_of_uint256 u =? z)%Z
+     then Some u
+     else None.
