UInt256.v
@@ -1,0 +1,37 @@
+From Coq Require Import ZArith.
+Require Import Config UntypedAST.
+
+Definition interpret_unop {C: VyperConfig} (op: unop) (a: uint256)
+: option uint256
+:= match op with
+   | BitwiseNot => Some (uint256_of_Z (Z.lxor (Z.ones 256) (Z_of_uint256 a)))
+   | Neg => maybe_uint256_of_Z (- Z_of_uint256 a) (* This only allows 0. *)
+   end.
+
+Definition interpret_binop {C: VyperConfig} (op: binop) (a b: uint256)
+: option uint256
+:= match op with
+   | Lt => Some (if (Z_of_uint256 a <?  Z_of_uint256 b)%Z then one256 else zero256)
+   | Le => Some (if (Z_of_uint256 a <=? Z_of_uint256 b)%Z then one256 else zero256)
+   | Gt => Some (if (Z_of_uint256 a >?  Z_of_uint256 b)%Z then one256 else zero256)
+   | Ge => Some (if (Z_of_uint256 a >=? Z_of_uint256 b)%Z then one256 else zero256)
+   | Eq => Some (if (Z_of_uint256 a =?  Z_of_uint256 b)%Z then one256 else zero256)
+   | Ne => Some (if (Z_of_uint256 a =?  Z_of_uint256 b)%Z then zero256 else one256)
+   | BitwiseOr  => Some (uint256_of_Z (Z.lor  (Z_of_uint256 a) (Z_of_uint256 b)))
+   | BitwiseAnd => Some (uint256_of_Z (Z.land (Z_of_uint256 a) (Z_of_uint256 b)))
+   | BitwiseXor => Some (uint256_of_Z (Z.lxor (Z_of_uint256 a) (Z_of_uint256 b)))
+   | ShiftLeft  => Some (uint256_of_Z (Z.shiftl (Z_of_uint256 a) (Z_of_uint256 b)))
+   | ShiftRight => Some (uint256_of_Z (Z.shiftr (Z_of_uint256 a) (Z_of_uint256 b)))
+   | Add => maybe_uint256_of_Z (Z_of_uint256 a + Z_of_uint256 b)%Z
+   | Sub => maybe_uint256_of_Z (Z_of_uint256 a - Z_of_uint256 b)%Z
+   | Mul => maybe_uint256_of_Z (Z_of_uint256 a * Z_of_uint256 b)%Z
+   | Quot => let bz := Z_of_uint256 b in
+             if (bz =? 0)%Z
+               then None
+               else maybe_uint256_of_Z (Z_of_uint256 a / bz)%Z
+   | Mod => let bz := Z_of_uint256 b in
+            if (bz =? 0)%Z
+               then None
+               else maybe_uint256_of_Z (Z_of_uint256 a mod bz)%Z
+   | Pow => maybe_uint256_of_Z (Z.pow (Z_of_uint256 a) (Z_of_uint256 b))%Z
+   end.
